drop restricting property from cstep transisions

src/theory/tools/promising/strongPostCondLib.sig
@@ -5,4 +5,6 @@ sig
   val strong_post_define_consts :  term -> unit
   val strong_post_proof : term -> unit
 
+  val calculate_terms : term -> term * term * term
+
 end
